wip on adding mm refs related predicates to the memory relation

ulib/FStar.HyperStack.ST.fst
@@ -34,7 +34,7 @@ private abstract let rid_last_component_pred (m1 m2:mem) :Type0
                  ((~ (m1 `contains_region` r)) /\ rid_last_component r < get_rid_ctr m1) ==>
 		 (~ (m2 `contains_region` r))
 
-(* Predicate for refs *)
+(* Predicate for eternal refs *)
 private abstract let eternal_refs_pred (m1 m2:mem) :Type0
   = forall (a:Type) (rel:preorder a) (r:HS.mreference a rel).
       {:pattern (m1 `HS.contains` r)}
@@ -46,12 +46,42 @@ private abstract let eternal_refs_pred (m1 m2:mem) :Type0
 	  else True
 	else True
 
+(* Predicate for next ref address in a region's heap *)
+private abstract let next_ref_addr_in_a_region_pred (m1 m2:mem) :Type0
+  = forall (r:HS.rid).{:pattern (m1 `contains_region` r); (m1 `contains_region` r)}
+                 (m1 `contains_region` r /\ m2 `contains_region` r) ==>
+		 (let h1 = Map.sel (HS.get_hmap m1) r in
+		  let h2 = Map.sel (HS.get_hmap m2) r in
+		  Heap.next_addr h1 <= Heap.next_addr h2)
+
+(* Predicate that an unused ref whose addr is less than the next addr remains unallocated *)
+private abstract let unused_ref_next_addr_pred (m1 m2:mem) :Type0
+  = forall (rid:HS.rid).{:pattern (m1 `contains_region` rid); (m1 `contains_region` rid)}
+                   (m1 `contains_region` rid /\ m2 `contains_region` rid) ==>
+		   (let h1 = Map.sel (HS.get_hmap m1) rid in
+		    (forall (a:Type0) (rel:preorder a) (r:HS.mreference a rel).{:pattern (r `HS.unused_in` m1)}
+		       (HS.frameOf r == rid /\ r `HS.unused_in` m1 /\ HS.as_addr r < Heap.next_addr h1) ==>
+		       (r `HS.unused_in` m2)))
+
+(* Predicate for mm refs *)
+private abstract let mm_refs_pred (m1 m2:mem) :Type0
+  = forall (a:Type) (rel:preorder a) (r:HS.mreference a rel).
+      {:pattern (m1 `HS.contains` r)}
+      if not (is_mm r) then True
+      else
+        if m1 `HS.contains` r then
+	  if m2 `HS.contains` r then rel (HS.sel m1 r) (HS.sel m2 r)
+	  else r `HS.unused_in` m2
+	else True
+
 (* The preorder is the conjunction of above predicates *)
 private abstract let mem_rel :relation mem
   = fun (m1 m2:mem) ->
-    eternal_region_pred m1 m2 /\ rid_ctr_pred m1 m2 /\ rid_last_component_pred m1 m2 /\ eternal_refs_pred m1 m2
+    eternal_region_pred m1 m2 /\ rid_ctr_pred m1 m2 /\ rid_last_component_pred m1 m2 /\ eternal_refs_pred m1 m2 /\
+    next_ref_addr_in_a_region_pred m1 m2 /\ unused_ref_next_addr_pred m1 m2 /\ mm_refs_pred m1 m2
+
 private abstract let mem_pre :preorder mem =
-  HS.lemma_rid_ctr_pred ();
+  HS.lemma_rid_ctr_pred (); HS.lemma_next_addr_contained_refs_addr ();
   mem_rel
 
 type mem_predicate = mem -> Type0
@@ -380,6 +410,7 @@ private let salloc_common (#a:Type) (#rel:preorder a) (init:a) (mm:bool)
   (ensures  (fun m0 s m1 -> is_stack_region (HS.frameOf s) /\ salloc_post init m0 s m1 /\ is_mm s == mm))
   = let m0 = gst_get () in
     let r, m1 = HS.alloc rel (get_tip m0) init mm m0 in
+    Heap.lemma_next_addr_alloc rel (Map.sel (get_hmap m0) (get_tip m0)) init mm;  //AR: to prove that next_addr in tip's heap increases (it is part of mem_rel)
     gst_put m1;
     assert (Set.equal (Map.domain (get_hmap m0)) (Map.domain (get_hmap m1)));
     HS.lemma_rid_ctr_pred ();  //AR: to prove that rid_last_component of r.id is < rid_ctr
@@ -414,7 +445,8 @@ let sfree (#a:Type) (#rel:preorder a) (r:mmmstackref a rel)
     let m1 = HS.free r m0 in
     assert (Set.equal (Map.domain (get_hmap m0)) (Map.domain (get_hmap m1)));
     Heap.lemma_distinct_addrs_distinct_preorders ();
-    Heap.lemma_distinct_addrs_distinct_mm ();    
+    Heap.lemma_distinct_addrs_distinct_mm ();
+    Heap.lemma_next_addr_free_mm (Map.sel (HS.get_hmap m0) (HS.get_tip m0)) (HS.as_ref r);  //AR: to prove that next_addr in tip's heap remains same (to satisfy the predicate in mm rel)
     gst_put m1
 
 let new_region (r0:rid)
@@ -475,6 +507,7 @@ private let ralloc_common (#a:Type) (#rel:preorder a) (i:rid) (init:a) (mm:bool)
   = if i <> HS.root then gst_recall (region_contains_pred i);
     let m0 = gst_get () in
     let r, m1 = HS.alloc rel i init mm m0 in
+    Heap.lemma_next_addr_alloc rel (Map.sel (HS.get_hmap m0) i) init mm;  //AR: to prove that next_addr in tip's heap remains same (to satisfy the predicate in mm rel)
     gst_put m1;
     assert (Set.equal (Map.domain (get_hmap m0)) (Map.domain (get_hmap m1)));
     HS.lemma_rid_ctr_pred ();
@@ -517,6 +550,7 @@ let rfree (#a:Type) (#rel:preorder a) (r:mmmref a rel)
     assert (Set.equal (Map.domain (get_hmap m0)) (Map.domain (get_hmap m1)));
     Heap.lemma_distinct_addrs_distinct_preorders ();
     Heap.lemma_distinct_addrs_distinct_mm ();    
+    Heap.lemma_next_addr_free_mm (Map.sel (HS.get_hmap m0) (HS.frameOf r)) (HS.as_ref r);  //AR: to prove that next_addr in tip's heap remains same (to satisfy the predicate in mm rel)
     gst_put m1
 
 unfold let assign_post (#a:Type) (#rel:preorder a) (r:mreference a rel) (v:a) m0 (_u:unit) m1 =
@@ -537,6 +571,7 @@ let op_Colon_Equals (#a:Type) (#rel:preorder a) (r:mreference a rel) (v:a)
     Heap.lemma_distinct_addrs_distinct_preorders ();
     Heap.lemma_distinct_addrs_distinct_mm ();
     Heap.lemma_upd_equals_upd_tot_for_contained_refs (get_hmap m0 `Map.sel` (HS.frameOf r)) (HS.as_ref r) v;
+    Heap.lemma_next_addr_upd (Map.sel (HS.get_hmap m0) (HS.frameOf r)) (HS.as_ref r) v;  //next_addr in ref's rid heap remains same
     gst_put m1
 
 unfold let deref_post (#a:Type) (#rel:preorder a) (r:mreference a rel) m0 x m1 =
@@ -604,10 +639,11 @@ type erid = r:rid{is_eternal_region r}
 
 type m_rref (r:erid) (a:Type) (b:preorder a) = x:mref a b{HS.frameOf x = r}
 
-unfold type stable_on_t (#i:erid) (#a:Type) (#b:preorder a)
-                        (r:m_rref i a b) (p:mem_predicate)
-  = forall h0 h1.{:pattern (p h0); b (HS.sel h0 r) (HS.sel h1 r)}
-            (p h0 /\ b (HS.sel h0 r) (HS.sel h1 r)) ==> p h1
+unfold type stable_on_t_common (#a:Type0)
+
+unfold type stable_on_t (#a:Type0) (#rel:preorder a) (r:mreference a rel) (p:mem_predicate)
+  = forall (h0 h1:mem).{:pattern (p h0); rel (HS.sel h0 r) (HS.sel h1 r)}
+                  (p h0 /\ rel (HS.sel h0 r) (HS.sel h1 r)) ==> p h1
 
 let mr_witness (#r:erid) (#a:Type) (#b:preorder a)
                (m:m_rref r a b) (p:mem_predicate)
@@ -650,6 +686,9 @@ let testify_forall_region_contains_pred (#c:Type) (#p:(c -> rid))
   = let p' (x:c) :mem_predicate = region_contains_pred (p x) in
     let s:squash (forall (x:c). witnessed (p' x)) = () in
     testify_forall s
+
+
+
 
 type ex_rid = erid
 
